\documentclass{article}
\usepackage{biblatex}
\addbibresource{references.bib}
\usepackage{amsmath}
\bibliography{references}
\RequirePackage[a4paper, left=1.5in,right=1.5in,top=1in,bottom=1in]{geometry}
\newcommand{\floor}[1]{\left\lfloor #1 \right\rfloor}
\newcommand{\ceil}[1]{\left\lceil #1 \right\rceil}
\renewcommand{\theequation}{A\arabic{equation}}
\begin{document}
\section*{Appendix A: Z(n,k) formula derivation}
We have the recurrence
\begin{equation}\label{zet-recurrence}
Z(n,k) = 2\floor{k/2} Z(n-1,k)+Z(n-1,k-1),
\end{equation}
with initial conditions $Z(0,k) = \delta_{0,k}$, valid for $1 \leq k \leq n$, which forms a lower triangular array. 
Here I derive an explicit formula for $Z(n,k)$. Let $A_k$ be the ordinary generating function for the k-th column over $x^n$:
$$
A_k(x) = \sum_{n} Z(n,k) x^n
$$
We first multiply each side of the recurrence in Eq. \ref{zet-recurrence} by $x^n$ and sum over n:
$$
\begin{aligned}
\sum_{n \geq 1} Z(n,k)x^n &= 2\floor{k/2}\sum_{n \geq 1}Z(n-1,k)x^n + \sum_{n \geq 1} Z(n-1,k-1) x^n \\
A_k -Z(0,k)&=2\floor{k/2}x A_k+x A_{k-1}, \quad k \geq 1
\end{aligned}
$$
Since $Z(0,k) = 0$ when $k \neq 0$, then this simplifies to the following recurrence for the column generating function:
$$
A_k = \frac{x}{(1-2\floor{k/2}x)} A_{k-1}
$$
We know from the initial conditions that $A_0(x) = 1$, hence:
$$
\begin{aligned}
    A_0 &= 1 \\
    A_1 &= x \\
    A_2 &= \frac{x^2}{1-2x} \\
    A_3 &= \frac{x^3}{(1-2x)^2} \\
    A_4 &= \frac{x^4}{(1-2x)^2 (1-4x)} \\
    A_5 &= \frac{x^5}{(1-2x)^2 (1-4x)^2}, \\
\end{aligned}
$$
and so on. More generally, the ordinary generating function for the k-th column is:
\begin{equation}\label{column-ogf}
A_k(x) = \frac{x^k}{\prod_{j=0}^k(1-2\floor{j/2}x)}
\end{equation}
In order to get an explicit formula for $Z(n,k)$, use the technique on p.19 of \cite{wilfGeneratingfunctionologyThirdEdition2005}:
$$
Z(n,k) = [x^n]A(x),
$$
where $[x^n]$ is the coefficient extractor operator. Start with partial fraction decomposition of $A_k(x)$. First, denote:
$$
A_k(x) = x^kP_k(x),
$$
where
$$
P_k(x) = \prod_{0 \leq j \leq k}\frac{1}{1-2\floor{j/2}x}.
$$
Hence
\begin{equation}\label{znk-coef}
Z(n,k) = [x^n]x^kP_k(x) = [x^{n-k}]P_k(x)
\end{equation}
We can express $P_k(x)$ as a sum of partial fractions with unknown coefficients (note the slight difference in ranges for odd and even k):

\begin{equation}\label{pkx}
    \begin{aligned}
    P_{2m}(x) &= \sum_{1 \leq j \leq m} \frac{C_{2m,j}}{1-2jx} + \sum_{1 \leq j \leq m-1} \frac{D_{2m,j}}{(1-2jx)^2} \\
    P_{2m+1}(x) &= \sum_{1 \leq j \leq m} \frac{C_{2m+1,j}}{1-2jx} + \sum_{1 \leq j \leq m} \frac{D_{2m+1,j}}{(1-2jx)^2}
    \end{aligned}
\end{equation}

It is easy to calculate the $D$ coefficients with the standard Heaviside cover-up method:
$$
\begin{aligned}
    D_{k,r} &= (1-2rx)^2P_k(x)|_{x=\frac{1}{2r}} \\
    &= (1-2rx)^2 \prod_{1 \leq j \leq k} \frac{1}{1-2 \floor{j/2}x} \bigg|_{x=\frac{1}{2r}} \\
    &= \prod_{1 \leq j < 2r} \frac{1}{1-\floor{j/2}/r} \prod_{2r < j \leq k} \frac{1}{1- \floor{j/2}/r} \\
    &= \prod_{1 \leq j < 2r} \frac{r}{r-\floor{j/2}} \prod_{2r < j \leq k} \frac{r}{r- \floor{j/2}}, \\
\end{aligned}
$$
which simplifies to:
\begin{equation}\label{d-k-r}
        D_{k,r}=\frac{(-r)^{k-1}}{r!r!(\floor{\frac{k}{2}}-r)!(\floor{\frac{k-1}{2}}-r)!}.
\end{equation}
$D_{k,r}$ varies only slightly for even and odd k:
$$
\begin{aligned}
    D_{2m,r} &= \frac{-r^{2m-1}}{r!r!(m-r)!(m-1-r)!} \\
    D_{2m+1,r} &= \frac{r^{2m}}{r!r!(m-r)!(m-r)!} \\
\end{aligned}
$$
For the $C_{k,j}$ coefficients, we have two main cases to consider. When $k=2m$ is even and $j=m$, $P_k(x)$ has a simple pole at $1-2mx$, so we get $C_{2m,m}$ easily by the same method:
\begin{equation}\label{c-2m-m}
    C_{2m,m} = (1-2mx)P_{2m}(x)|_{x=\frac{1}{2m}} = \frac{m^{2m}}{m!m!}
\end{equation}
For the remaining C coefficients  we have a pole of $P_k(x)$ of multiplicity 2 at $1-2jx$ so we need to use the derivative method. Specifically:
$$
-2r C_{k,r} = \frac{\mathrm{d}}{\mathrm{d}x} (1-2rx)^2P_k(x)\bigg|_{x=\frac{1}{2r}}
$$
Let 
$$
\begin{aligned}
Q_r &= (1-2rx)^2 P_k(x) = \prod_{j} \frac{1}{(1-2jx)^{e_j}},\\
e_j &= 
    \begin{cases} 
    2,& \mathrm{if}\quad 0 \leq 2j < k \land  j \neq r \\ 
    1, & \mathrm{if} \quad 2j = k \land j \neq r \\
    0, & \mathrm{otherwise}
    \end{cases}
\end{aligned}
$$
Then $C_{k,r} = -\frac{1}{2r}Q'_r\left (\frac{1}{2r} \right)$ and we can use the logarithmic derivative to simplify the calculation:

$$ 
\begin{aligned}
    \frac{Q'_{r}}{Q_r} &= \frac{d}{dx}log(Q_r) = \frac{d}{dx}\left[ -\sum_{j} e_j\log(1-2jx) \right]=  \sum_{j} 2e_j\frac{j}{1-2jx}  \\
    C_{k,r} &= - \frac{1}{2r}Q'_r\left (\frac{1}{2r} \right) = -\log(Q_r(x))'Q_r(x)|_{x=1/{2r}} \\
    &= -\frac{1}{2r} Q_r\left(\frac{1}{2r}\right) 2\sum_{j} e_j\frac{j}{1-j/r} \\ 
    &= -\frac{1}{2r} 2 D_{k,r}\sum_{j}e_j\frac{rj }{r-j} \\
    &= - \frac{1}{2r}2r D_{k,r}\sum_{j}e_j \frac{j}{r-j} \\
    &= - D_{k,r}\sum_{j}e_j \frac{j}{r-j} \\
\end{aligned}
$$
Let $S_k=\sum_{j}e_j\frac{j}{r-j}$ and simplify S. First, consider the case $k=2m+1$. 
$$
\begin{aligned}
    S_{2m+1} &=  2\sum_{\substack{1 \leq j \leq m \\ j \neq r}}\frac{j}{r-j} \\ 
    &= 2\left[\frac{1}{r-1}+\frac{2}{r-2} + \cdots  + \frac{r-1}{1}-\frac{r+1}{1}-\frac{r+2}{2}-\cdots-\frac{m}{m-r}\right]\\
    &= 2\sum_{1 \leq j \leq r-1}\frac{r-j}{j} -2\sum_{1 \leq j \leq m-r}\frac{j+r}{j} \\
    &= 2r\left(\sum_{1 \leq j \leq r-1}\frac{1}{j}\right) - 2(r-1) - 2r\left(\sum_{1 \leq j \leq m-r}\frac{1}{j}\right)-2(m-r)\\
    &= 2r(H_{r-1}-H_{m-r})-2m+2 \\
\end{aligned}
$$
where $H_n$ is the $n^{th}$ harmonic number. We proceed similarly for $k=2m$ with some care about $e_{m}=1$:
$$
\begin{aligned}
    S_{2m} &= \sum_{j}e_j \frac{j}{r-j} = \frac{m}{r-m} + 2\sum_{\substack{1 \leq j \leq m-1 \\ j \neq r}}\frac{j}{r-j}\\ 
    &= \frac{m}{r-m} + 2 \sum_{1 \leq j \leq r-1} \frac{j}{r-j} - 2\sum_{r+1 \leq j \leq m-1}\frac{j}{j-r} \\
    &= \frac{m}{r-m} + 2\sum_{1 \leq j \leq r-1}\frac{r-j}{j} -2\sum_{1 \leq j \leq m-r-1}\frac{j+r}{j} \\
    &= \frac{m}{r-m} + 2rH_{r-1}-2(r-1)-2rH_{m-r-1}-2(m-r-1) \\
    &=  2rH_{r-1} - 2rH_{m-r-1}-2(m-2)-\frac{m}{m-r}  \\
    &= 2rH_{r-1} - 2rH_{m-r-1} - 2(m-2) - \frac{r}{m-r} -1 \\
    &= r\left(2H_{r-1} - H_{m-r-1}-H_{m-r}\right) - 2m + 3
\end{aligned}
$$
Generally when $r \neq m$:
\begin{equation}\label{s-k}
    S_k = r(2H_{r-1}-H_{\floor{k/2}-r}-H_{\floor{(k-1)/2}-r})-k+3
\end{equation}
Combining everything we have:
\begin{equation}\label{d-s-c}
    \begin{aligned}
        D_{k,r} &= \frac{(-r)^{k-1}}{r!r!(\floor{k/2}-r)!(\floor{(k-1)/2}-r)!} \\
        S_{k,r} &= r(2H_{r-1}-H_{\floor{k/2}-r}-H_{\floor{(k-1)/2}-r})-k+3 \\
        C_{k,r} &= 
        \begin{cases}
            - D_{k,r} S_{k,r} & \text{if}\, 1 \leq r < k/2\\
            \frac{r^{2r}}{r!r!} & \text{if}\, r = k/2\\
            0 & \text{otherwise}
        \end{cases} 
    \end{aligned}
\end{equation}
Next, let us find an explicit formula for Z(n,k). From \ref{znk-coef} and \ref{pkx}:
$$
\begin{aligned}
    Z(n,k) &=[x^{n-k}]P_k(x) \\
    &= [x^{n-k}]\left[ \sum_{1 \leq j \leq \floor{k/2}} \frac{C_{k,j}}{1-2jx} + \sum_{1 \leq j \leq \floor{(k-1)/2}} \frac{D_{k,j}}{(1-2jx)^2} \right]\\
     &= \sum_{1 \leq j \leq \floor{k/2}}C_{k,j}[x^{n-k}]  \frac{1}{1-2jx} + \sum_{1 \leq j \leq \floor{(k-1)/2}} D_{k,j}[x^{n-k}]\frac{1}{(1-2jx)^2} \\ 
\end{aligned}
$$
We have the standard geometric series expansions:
$$
\begin{aligned}
     & [x^{n-k}]\frac{1}{1-2jx} = [x^{n-k}]\sum_{i\geq0}(2j)^ix^i = (2j)^{n-k}\\ 
     & [x^{n-k}]\frac{1}{(1-2jx)^2} = [x^{n-k}]\sum_{i\geq0}(i+1)(2j)^ix^i = (n-k+1)(2j)^{n-k}.\\ 
\end{aligned}
$$
Which results in the following final set of formulas valid for $n \geq 2, k \geq 2$:
\begin{equation}
    \begin{aligned}
        Z(n,k &)= \sum_{1 \leq j \leq \floor{\frac{k}{2}}}(2j)^{n-k}\left (C_{k,j} +D_{k,j}(n-k+1) \right )\\
            D_{k,r} &= \frac{(-r)^{k-1}}{r!r!(\floor{\frac{k}{2}}-r)!(\floor{\frac{k-1}{2}}-r)!} \\
            C_{k,r} &= \begin{cases}
                - D_{k,r} (r(2H_{r-1}-H_{\floor{\frac{k}{2}}-r}-H_{\floor{\frac{k-1}{2}}-r})-k+3) & \text{if} \, 1 \leq r < k/2\\
                \frac{r^{2r}}{r!r!} & \text{if}  \, r = k/2\\
                0 & \text{otherwise}
            \end{cases} 
    \end{aligned}
\end{equation}
\printbibliography
\end{document}